Implementation modelChecker

CertifyingDatalog/ModelChecking.lean
@@ -17,13 +17,18 @@ def partialGroundRule.isSafe (pgr: partialGroundRule τ i): Prop :=
 
 def rule.isSafe (r: rule τ): Prop := atomVariables r.head ⊆ collectResultsToFinset atomVariables r.body
 
-def partialGroundRuleFromRule (r: rule τ): partialGroundRule τ i :=
+def partialGroundRuleFromRule (r: rule τ) (i: interpretation τ): partialGroundRule τ i :=
   have members: ∀ (ga: groundAtom τ), ga ∈ [] → ga ∈ i:= by
     simp
   {head := r.head, groundedBody := [], ungroundedBody := r.body, members := members}
 
 def partialGroundRule.toRule (pgr: partialGroundRule τ i): rule τ :=
   {head:= pgr.head, body := (List.map (groundAtom.toAtom) pgr.groundedBody) ++ pgr.ungroundedBody}
+
+lemma partialGroundRuleToRuleInverseToFromRule (r: rule τ) (i: interpretation τ): r = partialGroundRule.toRule (partialGroundRuleFromRule r i) := by
+  unfold partialGroundRuleFromRule
+  unfold partialGroundRule.toRule
+  simp
 
 def partialGroundRule.isTrue (pgr: partialGroundRule τ i): Prop := ∀ (g: grounding τ), ruleTrue (ruleGrounding pgr.toRule g) i
 
@@ -110,6 +115,23 @@ def atomWithoutVariablesToGroundAtom (a: atom τ) (h: atomVariables a = ∅): gr
     apply a.term_length
 {symbol:= a.symbol, atom_terms := List.map (fun ⟨x, _h⟩ => termWithoutVariablesToConstant x (h x _h)) a.atom_terms.attach, term_length := term_length }
 
+lemma atomWithoutVariablesToGroundAtomOfGroundAtom (ga: groundAtom τ)(h: atomVariables ga.toAtom = ∅): atomWithoutVariablesToGroundAtom ga.toAtom h = ga :=
+by
+  cases ga with
+  | mk symbol terms term_length =>
+    unfold atomWithoutVariablesToGroundAtom
+    unfold groundAtom.toAtom
+    simp
+    apply List.ext_get
+    rw [List.length_map, List.length_attach, List.length_map]
+
+    intros n h1 h2
+    rw [List.get_map]
+    simp [List.get_map]
+    unfold termWithoutVariablesToConstant
+    simp
+
+
 def List.map_except_unit {A B: Type} (l: List A) (f: A → Except B Unit): Except B Unit :=
   match l with
   | [] => Except.ok ()
@@ -118,14 +140,220 @@ def List.map_except_unit {A B: Type} (l: List A) (f: A → Except B Unit): Excep
     | Except.ok () => List.map_except_unit tl f
     | Except.error b => Except.error b
 
-def getSubstitutions (i: List (groundAtom τ))(a: atom τ): List (substitution τ) := List.filterMap (fun x => matchAtom emptySubstitution a x) i
+lemma List.map_except_unitIsUnitIffAll {A B: Type} (l: List A) (f: A → Except B Unit): List.map_except_unit l f = Except.ok () ↔ ∀ (a:A), a ∈ l → f a = Except.ok () :=
+by
+  induction l with
+  | nil =>
+    simp
+    unfold List.map_except_unit
+    rfl
+  | cons hd tl ih =>
+    unfold List.map_except_unit
+    simp
+    cases f hd with
+    | ok u =>
+      simp
+      rw [ih]
+    | error e =>
+      simp
 
 def List.toSet {A: Type} (l: List A): Set A :=
   match l with
   | [] => ∅
   | hd::tl => {hd} ∪ tl.toSet
 
-def groundingStep (s: substitution τ) (i: List (groundAtom τ)) (pgr: partialGroundRule τ i.toSet ) (hd: atom τ) (tl: List (atom τ)) (ungroundedBody: pgr.ungroundedBody = hd::tl) (noVars: atomVariables (applySubstitutionAtom s hd) = ∅ ): partialGroundRule τ i.toSet := sorry
+lemma List.toSet_mem {A: Type} (a:A) (l: List A): a ∈ l ↔ a ∈ l.toSet := by
+  induction l with
+  | nil =>
+    unfold List.toSet
+    simp
+  | cons hd tl ih =>
+    unfold List.toSet
+    simp
+    rw [ih]
+
+def getSubstitutions (i: List (groundAtom τ))(a: atom τ): List (substitution τ) := List.filterMap (fun x => matchAtom emptySubstitution a x) i
+
+lemma collectResultsToFinsetEmptyIffAllMembersAre {A: Type} (f: A → Set τ.vars) (l: List A): collectResultsToFinset f l = ∅ ↔ ∀ (a:A), a ∈ l → f a = ∅ := by
+  induction l with
+  | nil =>
+    unfold collectResultsToFinset
+    simp
+  | cons hd tl ih =>
+    unfold collectResultsToFinset
+    rw [union_is_empty_iff_both]
+    rw [ih]
+    simp
+
+lemma groundAtomsHaveNoVariables (ga: groundAtom τ): atomVariables ga.toAtom = ∅ := by
+  cases ga with
+  | mk symbol atom_terms term_length =>
+    unfold atomVariables
+    unfold groundAtom.toAtom
+    simp
+    rw [collectResultsToFinsetEmptyIffAllMembersAre]
+    intros t t_map
+    rw [List.mem_map] at t_map
+    rcases t_map with ⟨c, _, c_t⟩
+    rw [← c_t]
+    unfold termVariables
+    simp
+
+lemma inGetSubstitutionsImplNoVars (i: List (groundAtom τ))(a: atom τ) (s: substitution τ) (h: s ∈ getSubstitutions i a): atomVariables (applySubstitutionAtom s a) = ∅ := by
+  unfold getSubstitutions at h
+  rw [List.mem_filterMap] at h
+  rcases h with ⟨ga, _, match_ga⟩
+  have matchAtomSome: Option.isSome (matchAtom emptySubstitution a ga) = true
+  rw [match_ga]
+  simp
+  have matchSemantic:applySubstitutionAtom (Option.get (matchAtom emptySubstitution a ga) matchAtomSome) a = ga
+  simp [matchAtomFindsSolution]
+
+  simp at matchSemantic
+  have matchAtom_s: Option.get (matchAtom emptySubstitution a ga) matchAtomSome= s
+  simp [match_ga]
+  rw [← matchAtom_s]
+  rw [matchSemantic]
+  apply groundAtomsHaveNoVariables
+
+lemma inGetSubstitutionsImplInInterpretation (i: List (groundAtom τ))(a: atom τ) (s: substitution τ) (h: s ∈ getSubstitutions i a)  (noVars: atomVariables (applySubstitutionAtom s a) = ∅): atomWithoutVariablesToGroundAtom (applySubstitutionAtom s a) noVars ∈ i :=
+by
+  unfold getSubstitutions at h
+  rw [List.mem_filterMap] at h
+  rcases h with ⟨ga, ga_i, match_ga⟩
+
+  have matchAtomSome: Option.isSome (matchAtom emptySubstitution a ga) = true
+  rw [match_ga]
+  simp
+  have matchSemantic:applySubstitutionAtom (Option.get (matchAtom emptySubstitution a ga) matchAtomSome) a = ga
+  simp [matchAtomFindsSolution]
+
+  simp at matchSemantic
+  have matchAtom_s: Option.get (matchAtom emptySubstitution a ga) matchAtomSome= s
+  simp [match_ga]
+
+  simp [← matchAtom_s]
+  simp [matchSemantic]
+  rw [atomWithoutVariablesToGroundAtomOfGroundAtom]
+  apply ga_i
+
+lemma applySubstitutionAtomRemovesDomainFromAtomVars (a: atom τ) (s: substitution τ): atomVariables (applySubstitutionAtom s a) = (atomVariables a) \ (substitution_domain s) :=
+by
+  unfold atomVariables
+  unfold applySubstitutionAtom
+  simp
+  rw [Set.ext_iff]
+  intro v
+  simp [collectResultsToFinsetMemberIffListMember]
+  constructor
+  intro h
+  rcases h with ⟨t, t_mem, v_t⟩
+  rw [← exists_and_right]
+  use t
+  rw [and_assoc]
+  constructor
+  apply t_mem
+  unfold applySubstitutionTerm at v_t
+  cases t with
+  | constant c =>
+    simp at v_t
+    unfold termVariables at v_t
+    simp at v_t
+  | variableDL v' =>
+    unfold termVariables at v_t
+    simp at v_t
+    by_cases h: Option.isSome (s v') = true
+    simp [h] at v_t
+    simp [h] at v_t
+    rw [v_t]
+    unfold termVariables
+    simp
+    unfold substitution_domain
+    simp
+    cases h':s v' with
+    | some o =>
+      rw [h'] at h
+      simp at h
+    | none =>
+      simp
+
+  intro h
+  rw [← exists_and_right] at h
+  rcases h with ⟨t, h_t⟩
+  use t
+  simp [h_t]
+  rcases h_t with ⟨left, v_dom⟩
+  rcases left with ⟨t_terms, v_t⟩
+  unfold applySubstitutionTerm
+  unfold termVariables
+  cases t with
+  | constant c =>
+    simp
+    unfold termVariables at v_t
+    simp at v_t
+  | variableDL v' =>
+    simp
+    unfold termVariables at v_t
+    simp at v_t
+    unfold substitution_domain at v_dom
+    rw [Set.mem_setOf] at v_dom
+    rw [v_t] at v_dom
+    simp [v_dom]
+    apply v_t
+
+
+
+
+
+
+def groundingStep (s: substitution τ) (i: List (groundAtom τ)) (pgr: partialGroundRule τ i.toSet ) (hd: atom τ) (tl: List (atom τ)) (noVars: atomVariables (applySubstitutionAtom s hd) = ∅ ) (mem: atomWithoutVariablesToGroundAtom (applySubstitutionAtom s hd) noVars ∈ i): partialGroundRule τ i.toSet :=
+  have h: ∀ (ga : groundAtom τ), ga ∈ List.concat pgr.groundedBody (atomWithoutVariablesToGroundAtom (applySubstitutionAtom s hd) noVars) → ga ∈ List.toSet i := by
+    intros ga
+    simp
+    intro h'
+    cases h' with
+    | inl ga_grounded =>
+      apply pgr.members ga ga_grounded
+    | inr ga_new =>
+      rw [ga_new]
+      rw [← List.toSet_mem]
+      apply mem
+  {head:= applySubstitutionAtom s pgr.head, groundedBody:= List.concat pgr.groundedBody (atomWithoutVariablesToGroundAtom (applySubstitutionAtom s hd) noVars) , ungroundedBody := List.map (fun x => applySubstitutionAtom s x) tl, members := h}
+
+def groundingStepPreservesSafety (s: substitution τ) (i: List (groundAtom τ)) (pgr: partialGroundRule τ i.toSet ) (hd: atom τ) (tl: List (atom τ)) (noVars: atomVariables (applySubstitutionAtom s hd) = ∅ ) (mem: atomWithoutVariablesToGroundAtom (applySubstitutionAtom s hd) noVars ∈ i) (safe: pgr.isSafe) (h: pgr.ungroundedBody = hd::tl ): (groundingStep s i pgr hd tl noVars mem).isSafe := by
+  unfold partialGroundRule.isSafe
+  unfold groundingStep
+  simp
+  rw [applySubstitutionAtomRemovesDomainFromAtomVars,collectResultsToFinsetSemantics, Set.subset_def]
+  simp
+  intros v v_head v_dom
+  unfold partialGroundRule.isSafe at safe
+  rw [collectResultsToFinsetSemantics, Set.subset_def] at safe
+  simp at safe
+  specialize safe v v_head
+  rcases safe with ⟨a, a_body, v_a⟩
+  rw [h] at a_body
+  simp at a_body
+  cases a_body with
+  | inl a_hd =>
+    rw [a_hd] at v_a
+    exfalso
+    rw [applySubstitutionAtomRemovesDomainFromAtomVars] at noVars
+    rw [Set.ext_iff] at noVars
+    specialize noVars v
+    simp at noVars
+    specialize noVars v_a
+    exact absurd noVars v_dom
+  | inr a_tl =>
+    use a
+    constructor
+    exact a_tl
+    rw [applySubstitutionAtomRemovesDomainFromAtomVars]
+    simp
+    constructor
+    apply v_a
+    apply v_dom
+
 
 def exploreGrounding (i: List (groundAtom τ)) (pgr: partialGroundRule τ i.toSet ) (safe: pgr.isSafe): Except String Unit :=
   match h: pgr.ungroundedBody with
@@ -145,6 +373,46 @@ def exploreGrounding (i: List (groundAtom τ)) (pgr: partialGroundRule τ i.toSe
     then Except.ok ()
     else Except.error "Error"
   | hd::tl =>
-    sorry
+    have noVars: ∀ (s: substitution τ), s ∈ getSubstitutions i hd → atomVariables (applySubstitutionAtom s hd) = ∅ := by
+      apply inGetSubstitutionsImplNoVars
+
+
+    List.map_except_unit (getSubstitutions i hd).attach (fun ⟨s, _h⟩ => exploreGrounding i (groundingStep s i pgr hd tl (noVars s _h) (inGetSubstitutionsImplInInterpretation i hd s _h (noVars s _h))) (groundingStepPreservesSafety s i pgr hd tl (noVars s _h) (inGetSubstitutionsImplInInterpretation i hd s _h (noVars s _h)) safe h) )
+termination_by exploreGrounding i pgr safe => pgr.ungroundedBody.length
+decreasing_by
+  simp_wf
+  unfold groundingStep
+  simp
+  rw [h]
+  simp
+
 
 theorem exploreGroundingSemantics (i: List (groundAtom τ)) (pgr: partialGroundRule τ i.toSet ) (safe: pgr.isSafe): exploreGrounding i pgr safe = Except.ok () ↔ pgr.isTrue := sorry
+
+lemma safePreservedBetweenRuleAndPartialGroundRule (r: rule τ) (i: interpretation τ): r.isSafe ↔ (partialGroundRuleFromRule r i).isSafe := by
+  unfold partialGroundRule.isSafe
+  unfold rule.isSafe
+  unfold partialGroundRuleFromRule
+  simp
+
+def modelChecker (i: List (groundAtom τ)) (P: List (rule τ)) (safe: ∀ (r: rule τ), r ∈ P → r.isSafe): Except String Unit :=
+  have safe': ∀ (r: rule τ), r ∈ P → (partialGroundRuleFromRule r i.toSet ).isSafe := by
+    intros r rP
+    rw [← safePreservedBetweenRuleAndPartialGroundRule]
+    apply safe r rP
+  List.map_except_unit P.attach (fun ⟨x, _h⟩ => exploreGrounding i (partialGroundRuleFromRule x i.toSet ) (safe' x _h) )
+
+theorem modelCheckerUnitIffAllRulesTrue (i: List (groundAtom τ)) (P: List (rule τ)) (safe: ∀ (r: rule τ), r ∈ P → r.isSafe): modelChecker i P safe = Except.ok () ↔ (∀ (r: groundRule τ), r ∈ groundProgram P.toFinset → ruleTrue r i.toSet) :=
+by
+  unfold modelChecker
+  rw [List.map_except_unitIsUnitIffAll]
+  simp [exploreGroundingSemantics, partialGroundRule.isTrue, groundProgram, ← partialGroundRuleToRuleInverseToFromRule]
+  constructor
+  intros h gr r rP g gr_r
+  rw [gr_r]
+  apply h r rP
+
+  intros h r rP g
+  specialize h (ruleGrounding r g)
+  apply h r rP g
+  rfl
